case_studies/tests/output/tests/proofs/proof_iterator_test_iterator_2.v
@@ -19,9 +19,9 @@ Proof.
   Unshelve. all: sidecond_hammer.
   { rename select (Forall2 _ _ _) into Hf.
     opose proof* Forall2_length as Hlen; first apply Hf.
-    do 11 (try destruct x' as [ | ? x']; simpl in *; first try lia); last lia. 
+    do 11 (try destruct x' as [ | ? x']; simpl in *; first try lia); last lia.
     apply Forall2_Forall2_cb in Hf.
-    move: Hf. simpl. 
+    move: Hf. cbn.
     naive_solver. }
   Unshelve. all: print_remaining_sidecond.
 Qed.
